<?xml version="1.0"?>

<rdf:RDF
    xmlns:dct="http://purl.org/dc/terms/"
    xmlns:rdf="http://www.w3.org/1999/02/22-rdf-syntax-ns#"
    xmlns:xsd="http://www.w3.org/2001/XMLSchema#"
    xmlns:rdfs="http://www.w3.org/2000/01/rdf-schema#"
    xmlns:owl="http://www.w3.org/2002/07/owl#"
    xmlns:akt="http://www.aktors.org/ontology/portal#"
    xmlns:daml="http://www.daml.org/2001/03/daml+oil#"
    xmlns:dc="http://purl.org/dc/elements/1.1/"
    xmlns="http://courseware.rkbexplorer.com/ontologies/courseware#"
  xml:base="http://courseware.rkbexplorer.com/ontologies/courseware">
  
  <owl:Ontology rdf:about="">
    <rdfs:label>ReSIST Courseware Ontology</rdfs:label>
    <dc:title xml:lang="en">ReSIST Courseware Ontology</dc:title>
    <dc:description xml:lang="en">The ReSIST Courseware Ontology represents the various eduacational courses and resources within the ReSIST project</dc:description>
    <owl:versionInfo>0.1</owl:versionInfo>
    <dc:creator>Bene Rodriguez</dc:creator>
    <dc:creator>Ian Millard</dc:creator>
    <dc:created>2006-05-03</dc:created>
    <owl:imports rdf:resource="http://www.aktors.org/ontology/portal"/>
  </owl:Ontology>

  <owl:Class rdf:ID="Student-Interaction-Type">
    <rdfs:comment>A type of interaction in which a student engages whilst undertaking a course; instances of this class may include lectures, laboratory sessions, and group or individual projects.</rdfs:comment>
    <rdfs:label>Student Interaction Type</rdfs:label>
    <rdfs:isDefinedBy rdf:resource="" />
  </owl:Class>
  
  <owl:Class rdf:ID="Pre-requisite">
    <rdfs:comment>This class encapsulates a body of previous knowledge required to undertake a course.</rdfs:comment>
    <rdfs:label>Pre-requisite</rdfs:label>
    <rdfs:isDefinedBy rdf:resource="" />
  </owl:Class>
  
  <owl:Class rdf:ID="Course">
    <rdfs:comment>This class encapsulates a course that is taught to students</rdfs:comment>
    <rdfs:label>Course</rdfs:label>
    <rdfs:subClassOf rdf:resource="http://www.aktors.org/ontology/portal#Abstract-Information"/>
    <rdfs:isDefinedBy rdf:resource="" />
  </owl:Class>
  
  <owl:DatatypeProperty rdf:ID="has-title">
    <rdfs:range rdf:resource="http://www.w3.org/2001/XMLSchema#string"/>
    <rdfs:label>title</rdfs:label>
    <rdfs:domain rdf:resource="#Course"/>
    <rdfs:comment>The title of this course</rdfs:comment>
    <rdfs:subPropertyOf rdf:resource="http://www.w3.org/2000/01/rdf-schema#label" />
    <rdfs:isDefinedBy rdf:resource="" />
  </owl:DatatypeProperty>
  
  <owl:Class rdf:ID="Assessment-Method">
    <rdfs:comment>A method by which a student is assessed; instances of this class may include examination, coursework, etc.</rdfs:comment>
    <rdfs:label>Assessment Method</rdfs:label>
    <rdfs:isDefinedBy rdf:resource="" />
  </owl:Class>
  
  <owl:ObjectProperty rdf:ID="has-courseware">
    <rdfs:comment>Courseware used by the Resist-Course (reference texts, personal hand-outs, slides, etc).</rdfs:comment>
    <rdfs:label>has courseware</rdfs:label>
    <rdfs:range rdf:resource="http://www.aktors.org/ontology/portal#Publication-Reference"/>
    <rdfs:domain rdf:resource="#Course"/>
    <rdfs:isDefinedBy rdf:resource="" />
  </owl:ObjectProperty>
  
  <owl:ObjectProperty rdf:ID="submitted-by">
    <rdfs:range rdf:resource="http://www.aktors.org/ontology/portal#Generic-Agent"/>
    <rdfs:domain rdf:resource="#Course"/>
    <rdfs:label>submitted by</rdfs:label>
    <rdfs:comment>The ReSIST Project member who has submitted and is the point of contact for this course</rdfs:comment>
    <rdfs:isDefinedBy rdf:resource="" />
  </owl:ObjectProperty>
  
  <owl:ObjectProperty rdf:ID="has-assessment-method">
    <rdfs:domain rdf:resource="#Course"/>
    <rdfs:range rdf:resource="#Assessment-Method"/>
    <rdfs:label>has assessment method</rdfs:label>
    <rdfs:isDefinedBy rdf:resource="" />
  </owl:ObjectProperty>
  
  <owl:ObjectProperty rdf:ID="has-prerequisite">
    <rdfs:domain rdf:resource="#Course"/>
    <rdfs:label>has pre-requisite</rdfs:label>
    <rdfs:range rdf:resource="#Pre-requisite"/>
    <rdfs:isDefinedBy rdf:resource="" />
  </owl:ObjectProperty>
  
  <owl:ObjectProperty rdf:ID="involves-organization">
    <rdfs:domain rdf:resource="#Course"/>
    <rdfs:label>involves organisation</rdfs:label>
    <rdfs:range rdf:resource="http://www.aktors.org/ontology/portal#Organization"/>
    <rdfs:comment>The association of an organisation which is involved in delivering a course</rdfs:comment>
    <rdfs:isDefinedBy rdf:resource="" />
  </owl:ObjectProperty>
  
  <owl:ObjectProperty rdf:ID="has-student-interaction-type">
    <rdfs:range rdf:resource="#Student-Interaction-Type"/>
    <rdfs:label>has student interaction type</rdfs:label>
    <rdfs:comment>Identifies a course as having the prescribed interaction type</rdfs:comment>
    <rdfs:domain rdf:resource="#Course"/>
    <rdfs:isDefinedBy rdf:resource="" />
  </owl:ObjectProperty>
  
  <owl:ObjectProperty rdf:ID="has-rights">
    <rdfs:domain rdf:resource="http://www.aktors.org/ontology/portal#Abstract-Information"/>
    <rdfs:comment>This property describes the intellectual property rights and conditions of use for this learning object. </rdfs:comment>
    <rdfs:isDefinedBy rdf:resource="" />
  </owl:ObjectProperty>
  
  <owl:ObjectProperty rdf:ID="has-infrastructure-requirement">
    <rdfs:range rdf:resource="http://www.aktors.org/ontology/portal#Technology"/>
    <rdfs:domain rdf:resource="#Course"/>
    <rdfs:label>has infrastructure requirement</rdfs:label>
    <rdfs:comment>An infrastructure requirement that is needed to carry out the course</rdfs:comment>
    <rdfs:isDefinedBy rdf:resource="" />
  </owl:ObjectProperty>
  
  <owl:ObjectProperty rdf:ID="taught-at">
    <rdfs:domain rdf:resource="#Course"/>
    <rdfs:label>taught at</rdfs:label>
    <rdfs:range rdf:resource="http://www.aktors.org/ontology/portal#Organization"/>
    <rdfs:comment>The organization at which this course is taught</rdfs:comment>
    <rdfs:isDefinedBy rdf:resource="" />
  </owl:ObjectProperty>
  
  <owl:ObjectProperty rdf:ID="has-instructor">
    <rdfs:label>has instructor</rdfs:label>
    <rdfs:domain rdf:resource="#Course"/>
    <rdfs:comment>A person delivering tuition as part of the course</rdfs:comment>
    <rdfs:range rdf:resource="http://www.aktors.org/ontology/portal#Person"/>
    <rdfs:isDefinedBy rdf:resource="" />
  </owl:ObjectProperty>
  
  <owl:ObjectProperty rdf:ID="has-author">
    <rdfs:range rdf:resource="http://www.aktors.org/ontology/portal#Generic-Agent"/>
    <rdfs:domain rdf:resource="#Course"/>
    <rdfs:label>has author</rdfs:label>
    <rdfs:comment>A person which is involved with the creation of the course</rdfs:comment>
    <rdfs:isDefinedBy rdf:resource="" />
  </owl:ObjectProperty>
  
  <owl:DatatypeProperty rdf:ID="course-objectives">
    <rdfs:range rdf:resource="http://www.w3.org/2001/XMLSchema#string"/>
    <rdfs:label>course objectives</rdfs:label>
    <rdfs:domain rdf:resource="#Course"/>
    <rdfs:comment>The objectives of this course</rdfs:comment>
    <rdfs:isDefinedBy rdf:resource="" />
  </owl:DatatypeProperty>
  
  <owl:DatatypeProperty rdf:ID="detailed-description">
    <rdfs:label>detailed description</rdfs:label>
    <rdfs:comment>A detailed description of the content conveyed within the course</rdfs:comment>
    <rdfs:domain rdf:resource="#Course"/>
    <rdfs:range rdf:resource="http://www.w3.org/2001/XMLSchema#string"/>
    <rdfs:isDefinedBy rdf:resource="" />
  </owl:DatatypeProperty>
  
  <owl:DatatypeProperty rdf:ID="hours-of-labs">
    <rdfs:domain rdf:resource="#Course"/>
    <rdfs:label>hours of labs</rdfs:label>
    <rdfs:range rdf:resource="http://www.w3.org/2001/XMLSchema#float"/>
    <rdfs:comment>The total number of hours of laboratory sessions in this course</rdfs:comment>
    <rdfs:isDefinedBy rdf:resource="" />
  </owl:DatatypeProperty>
  
  <owl:DatatypeProperty rdf:ID="has-rights-cost">
    <rdfs:comment>Whether use of this learning resource requires payment</rdfs:comment>
    <rdfs:domain rdf:resource="http://www.aktors.org/ontology/portal#Abstract-Information"/>
    <rdfs:range>
      <owl:DataRange>
        <owl:oneOf rdf:parseType="Resource">
          <rdf:first>false</rdf:first>
          <rdf:rest rdf:parseType="Resource">
            <rdf:rest rdf:resource="http://www.w3.org/1999/02/22-rdf-syntax-ns#nil"/>
            <rdf:first>true</rdf:first>
          </rdf:rest>
        </owl:oneOf>
      </owl:DataRange>
    </rdfs:range>
    <rdfs:isDefinedBy rdf:resource="" />
  </owl:DatatypeProperty>
  
  <owl:DatatypeProperty rdf:ID="course-duration">
    <rdfs:comment>The total duration of the course (in hours)</rdfs:comment>
    <rdfs:range rdf:resource="http://www.w3.org/2001/XMLSchema#integer"/>
    <rdfs:label>course duration</rdfs:label>
    <rdfs:domain rdf:resource="#Course"/>
    <rdfs:isDefinedBy rdf:resource="" />
  </owl:DatatypeProperty>
  
  <owl:DatatypeProperty rdf:ID="has-language">
    <rdfs:label>has language</rdfs:label>
    <rdfs:domain rdf:resource="http://www.aktors.org/ontology/portal#Abstract-Information"/>
    <rdfs:comment>The language in which an item of abstract information is written, expressed or delivered.</rdfs:comment>
    <rdfs:range rdf:resource="http://www.w3.org/2001/XMLSchema#language"/>
    <rdfs:isDefinedBy rdf:resource="" />
  </owl:DatatypeProperty>
  
  <owl:DatatypeProperty rdf:ID="hours-of-personal-study">
    <rdfs:range rdf:resource="http://www.w3.org/2001/XMLSchema#float"/>
    <rdfs:label>hours of personal study</rdfs:label>
    <rdfs:domain rdf:resource="#Course"/>
    <rdfs:comment>The total number of hours of personal study in this course</rdfs:comment>
    <rdfs:isDefinedBy rdf:resource="" />
  </owl:DatatypeProperty>
  
  <owl:DatatypeProperty rdf:ID="hours-of-lectures">
    <rdfs:domain rdf:resource="#Course"/>
    <rdfs:range rdf:resource="http://www.w3.org/2001/XMLSchema#float"/>
    <rdfs:comment>The total number of hours of lectures delivered in this course</rdfs:comment>
    <rdfs:label>hours of lectures</rdfs:label>
    <rdfs:isDefinedBy rdf:resource="" />
  </owl:DatatypeProperty>
  
  <owl:DatatypeProperty rdf:ID="has-rights-copyright">
    <rdfs:range>
      <owl:DataRange>
        <owl:oneOf rdf:parseType="Resource">
          <rdf:rest rdf:parseType="Resource">
            <rdf:rest rdf:resource="http://www.w3.org/1999/02/22-rdf-syntax-ns#nil"/>
            <rdf:first>true</rdf:first>
          </rdf:rest>
          <rdf:first>false</rdf:first>
        </owl:oneOf>
      </owl:DataRange>
    </rdfs:range>
    <rdfs:domain rdf:resource="http://www.aktors.org/ontology/portal#Abstract-Information"/>
    <rdfs:comment>Whether copyright or other restrictions apply to the use of this learning resource.</rdfs:comment>
    <rdfs:isDefinedBy rdf:resource="" />
  </owl:DatatypeProperty>
  
  <owl:DatatypeProperty rdf:ID="is-taught-present">
    <rdfs:range>
      <owl:DataRange>
        <owl:oneOf rdf:parseType="Resource">
          <rdf:rest rdf:parseType="Resource">
            <rdf:rest rdf:resource="http://www.w3.org/1999/02/22-rdf-syntax-ns#nil"/>
            <rdf:first>true</rdf:first>
          </rdf:rest>
          <rdf:first>false</rdf:first>
        </owl:oneOf>
      </owl:DataRange>
    </rdfs:range>
    <rdfs:domain rdf:resource="#Course"/>
    <rdfs:isDefinedBy rdf:resource="" />
  </owl:DatatypeProperty>
  
  <owl:DatatypeProperty rdf:ID="has-rights-description">
    <rdfs:range rdf:resource="http://www.w3.org/2001/XMLSchema#string"/>
    <rdfs:domain rdf:resource="http://www.aktors.org/ontology/portal#Abstract-Information"/>
    <rdfs:comment>Comments on the conditions of use of this learning resource.</rdfs:comment>
    <rdfs:isDefinedBy rdf:resource="" />
  </owl:DatatypeProperty>
  
  <owl:DatatypeProperty rdf:ID="number-of-credits">
    <rdfs:label>number of credits</rdfs:label>
    <rdfs:domain rdf:resource="#Course"/>
    <rdfs:comment>The number of EU BS/MS program credits</rdfs:comment>
    <rdfs:range rdf:resource="http://www.w3.org/2001/XMLSchema#float"/>
    <rdfs:isDefinedBy rdf:resource="" />
  </owl:DatatypeProperty>
  
  <owl:DatatypeProperty rdf:ID="total-hours-engagement">
    <rdfs:label>total hours of engagement</rdfs:label>
    <rdfs:range rdf:resource="http://www.w3.org/2001/XMLSchema#float"/>
    <rdfs:domain rdf:resource="#Course"/>
    <rdfs:comment>The total number of hours of engagement while undertaking this course</rdfs:comment>
    <rdfs:isDefinedBy rdf:resource="" />
  </owl:DatatypeProperty>
  
</rdf:RDF>

<!-- Created with Protege (with OWL Plugin 2.1, Build 284)  http://protege.stanford.edu -->
<!-- 2007-04-18 br205r Edited manually. Removed references to "Prerequisite" class. Left references to "Pre-requisite" class only -->
<!-- 2011-02-14 icm    Added rdfs:isDefinedBy -->
